verify/DirectedCompute.v
@@ -10,35 +10,35 @@ Module DirectedCompute (Ctx : Ctx).
 
 Definition dtape : Type := dir * list Sym * list Sym.
 
-Definition undir (d : dtape) : ctape :=
+Definition undir (d : dtape) : tape :=
   match d with
   | (L, l, r) =>
     match l with
-    | s :: l => l {{s}} r
-    | [] => [] {{s0}} r
+    | s :: l => to_dlist l {{s}} to_dlist r
+    | [] => <[] {{s0}} to_dlist r
     end
   | (R, l, r) =>
     match r with
-    | s :: r => l {{s}} r
-    | [] => l {{s0}} []
+    | s :: r => to_dlist l {{s}} to_dlist r
+    | [] => to_dlist l {{s0}} []>
     end
   end.
 
 Lemma flip_undir : forall q d l r,
-  flip_conf (lift (q, undir (d, l, r))) = lift (q, undir (flip_dir d, r, l)).
+  flip_conf (q;; undir (d, l, r)) = q;; undir (flip_dir d, r, l).
 Proof.
   introv.
   destruct d.
-  - destruct l; reflexivity.
-  - destruct r; reflexivity.
+  - destruct l; simpl; repeat rewrite dflip_to_dlist; reflexivity.
+  - destruct r; simpl; repeat rewrite dflip_to_dlist; reflexivity.
 Qed.
 
 Lemma undir_left_s0 : forall n r,
-  undir (L, repeat s0 n, r) = (repeat s0 (pred n), s0, r).
-Proof. introv. destruct n; reflexivity. Qed.
+  undir (L, repeat s0 n, r) = (drepeat s0 (pred n), s0, to_dlist r).
+Proof. introv. destruct n; simpl; try rewrite to_dlist_repeat; reflexivity. Qed.
 
 Lemma undir_right_s0 : forall n l,
-  undir (R, l, repeat s0 n) = (l, s0, repeat s0 (pred n)).
-Proof. introv. destruct n; reflexivity. Qed.
+  undir (R, l, repeat s0 n) = (to_dlist l, s0, drepeat s0 (pred n)).
+Proof. introv. destruct n; simpl; try rewrite to_dlist_repeat; reflexivity. Qed.
 
 End DirectedCompute.
