verify/DirectedList.v
@@ -1,0 +1,131 @@
+(** * DirectedList: Lists that have a notion of direction. *)
+
+(**
+ * We want to represent the two sides of a Turing machine's tape as lists,
+ * with the first element being the one closest to the machine head. This
+ * yields a nice formulation, with one issue: the first element will always get
+ * printed first by Coq.
+
+ * With some notation hacks, it would be possible to at least have Coq
+ * understand us when we write a list "backwards", but there's no way to have
+ * it use the direction we'd like in its responses – trust me, I've tried it
+ * all.
+
+ * The solution is to have the left and right side of the tape be separate
+ * types, even if only differing by an irrelevant type parameter. *)
+
+From Coq Require Import JMeq.
+From Coq Require Import List. Import ListNotations.
+From BusyCoq Require Export Helper.
+Set Default Goal Selector "!".
+
+Infix "==" := JMeq (at level 70, no associativity).
+
+Inductive dir : Type := L | R.
+
+Definition flip_dir (d : dir) :=
+  match d with
+  | L => R
+  | R => L
+  end.
+
+Lemma flip_dir_involutive : forall d,
+  flip_dir (flip_dir d) = d.
+Proof. intros []; reflexivity. Qed.
+
+Inductive dlist (A : Type) (d : dir) : Type :=
+  | dnil : dlist A d
+  | dcons : A -> dlist A d -> dlist A d.
+Arguments dnil {A} {d}.
+Arguments dcons {A} {d}.
+
+(* [dlist A L] grows to the left, so the head of the list is on the right.
+ * Likewise, [dlist A R] grows to the right, so the head of the list is on
+ * the left. *)
+
+Notation "xs <: x" := (@dcons _ L x xs) (at level 61, left associativity).
+Notation "x :> xs" := (@dcons _ R x xs) (at level 60, right associativity).
+Notation "< [ ]" := (@dnil _ L) (format "< [ ]").
+Notation "[ ] >" := (@dnil _ R) (format "[ ] >").
+
+Notation "< [ x ; .. ; y ]" := (dcons y .. (dcons x <[]) ..)
+  (format "< [ '[' x ;  '/' .. ;  '/' z ']' ]").
+Notation "[ x ; .. ; y ] >" := (dcons x .. (dcons y []>) ..)
+  (format "[ '[' x ;  '/' .. ;  '/' z ']' ] >").
+
+Fixpoint to_dlist {A} {d} (xs : list A) : dlist A d :=
+  match xs with
+  | [] => dnil
+  | x :: xs => dcons x (to_dlist xs)
+  end.
+
+Fixpoint dflip {A} {d} (xs : dlist A d) : dlist A (flip_dir d) :=
+  match xs with
+  | dnil => dnil
+  | dcons x xs => dcons x (dflip xs)
+  end.
+
+Lemma dflip_involutive : forall {A} d (xs : dlist A d),
+  dflip (dflip xs) == xs.
+Proof.
+  destruct d; simpl flip_dir; induction xs; simpl; try rewrite IHxs; auto.
+Qed.
+
+Lemma dflip_to_dlist : forall A d (xs : list A),
+  @dflip _ d (to_dlist xs) = to_dlist xs.
+Proof.
+  induction xs; simpl; congruence.
+Qed.
+
+Fixpoint app {A} {d} (xs ys : dlist A d) : dlist A d :=
+  match xs with
+  | dnil => ys
+  | dcons x xs => dcons x (app xs ys)
+  end.
+
+Notation "ys <+ xs" := (@app _ L xs ys) (at level 61, left associativity).
+Notation "xs +> ys" := (@app _ R xs ys) (at level 60, right associativity).
+
+Definition tl {A} {d} (xs : dlist A d) : dlist A d :=
+  match xs with
+  | dnil => dnil
+  | dcons x xs => xs
+  end.
+
+Fixpoint drepeat {A} {d} (x : A) (n : nat) : dlist A d :=
+  match n with
+  | O => dnil
+  | S n => dcons x (drepeat x n)
+  end.
+
+Lemma to_dlist_repeat : forall A d (x : A) n,
+  @to_dlist _ d (repeat x n) = drepeat x n.
+Proof.
+  induction n; simpl; congruence.
+Qed.
+
+Fixpoint dfirstn {A} {d} (n : nat) (xs : dlist A d) : dlist A d :=
+  match n with
+  | O => dnil
+  | S n =>
+    match xs with
+    | dnil => dnil
+    | dcons x xs => dcons x (dfirstn n xs)
+    end
+  end.
+
+Arguments dfirstn : simpl nomatch.
+
+Lemma dfirstn_less : forall n k A d (xs ys : dlist A d),
+  dfirstn (n + k) xs = dfirstn (n + k) ys ->
+  dfirstn n xs = dfirstn n ys.
+Proof.
+  induction n; introv H.
+  - reflexivity.
+  - destruct xs as [| x xs]; destruct ys as [| y ys];
+    simpl in H; try (discriminate || reflexivity).
+    simpl. inverts H as H. apply IHn in H.
+    congruence.
+Qed.
+
+#[export] Hint Resolve dfirstn_less : core.
