verify/TranslatedCyclers.v
@@ -12,101 +12,12 @@ Set Default Goal Selector "!".
 Module TranslatedCyclers (Ctx : Ctx).
   Module Flip := Flip Ctx. Export Flip.
 
-(** [EqTake] holds if the first [n] symbols on a particular side of the
-    tape match. *)
-Fixpoint EqTake (n : nat) (xs ys : side): Prop :=
-  match n with
-  | 0 => True
-  | S n =>
-    match xs, ys with
-    | Cons x xs, Cons y ys => x = y /\ EqTake n xs ys
-    end
-  end.
-
-Arguments EqTake !n !xs !ys.
-Arguments firstn [A] !n !l.
-
-Lemma EqTake_0 : forall xs ys, EqTake 0 xs ys.
-Proof. constructor. Qed.
-Local Hint Immediate EqTake_0 : core.
-
-Lemma EqTake_refl : forall n xs, EqTake n xs xs.
-Proof.
-  induction n; introv.
-  - exact I.
-  - destruct xs as [x xs].
-    simpl. auto.
-Qed.
-Local Hint Immediate EqTake_refl : core.
-
-Lemma EqTake_sym : forall n xs ys,
-  EqTake n xs ys -> EqTake n ys xs.
-Proof.
-  induction n; introv H.
-  - exact I.
-  - destruct xs, ys.
-    simpl. simpl in *.
-    destruct H. auto.
-Qed.
-
-Corollary EqTake_sym_iff : forall n xs ys,
-  EqTake n xs ys <-> EqTake n ys xs.
-Proof. introv. split; auto using EqTake_sym. Qed.
-
-Lemma EqTake_trans : forall n xs ys zs,
-  EqTake n xs ys -> EqTake n ys zs -> EqTake n xs zs.
-Proof.
-  induction n; introv H1 H2.
-  - exact I.
-  - destruct xs, ys, zs.
-    simpl. simpl in *.
-    destruct H1, H2. split.
-    + congruence.
-    + eauto.
-Qed.
-
-Lemma EqTake_less : forall n k xs ys,
-  EqTake (n + k) xs ys -> EqTake n xs ys.
-Proof.
-  induction n; introv H.
-  - exact I.
-  - destruct xs, ys.
-    simpl. simpl in H. destruct H as [E H].
-    split; try assumption.
-    eapply IHn, H.
-Qed.
-
-Local Hint Immediate EqTake_less : core.
-
-Lemma EqTake_firstn : forall n xs ys,
-  EqTake n (lift_side xs) (lift_side ys) <->
-    lift_side (firstn n xs) = lift_side (firstn n ys).
-Proof with intuition; congruence.
-  induction n.
-  - introv. split; auto.
-  - introv. destruct xs; destruct ys; simpl.
-    + split; auto.
-    + rewrite const_unfold. simpl.
-      rewrite (IHn []), firstn_nil. simpl...
-    + rewrite const_unfold. simpl.
-      rewrite (IHn _ []), firstn_nil. simpl...
-    + rewrite IHn...
-Qed.
-
-Local Hint Resolve -> EqTake_firstn : core.
-Local Hint Resolve <- EqTake_firstn : core.
-
-Program Definition eqb_take (n : nat) (xs ys : list Sym)
-    : {EqTake n (lift_side xs) (lift_side ys)}
-      + {~ EqTake n (lift_side xs) (lift_side ys)} :=
-  Reduce (eqb_side (firstn n xs) (firstn n ys)).
-
 (** [EqLimit] checks that the tapes match if you don't look more
     than [n] steps left. *)
 Definition EqLimit (n : nat) (t t' : tape): Prop :=
   match t, t' with
   | l {{s}} r, l' {{s'}} r' =>
-    EqTake n l l' /\ s = s' /\ r = r'
+    dfirstn n l = dfirstn n l' /\ s = s' /\ r = r'
   end.
 
 Local Hint Unfold EqLimit : core.
@@ -116,11 +27,11 @@ Lemma EqLimit_move_left : forall n t t',
   EqLimit n (move_left t) (move_left t').
 Proof.
   introv H.
-  destruct t as [[[u l] s] r].
-  destruct t' as [[[u' l'] s'] r'].
-  simpl in H. simpl.
-  destruct H as [[Eu El] [Es Er]].
-  repeat split; try assumption; congruence.
+  destruct t as [[[| u l] s] r];
+    destruct t' as [[[| u' l'] s'] r'];
+    destruct H as [Hl [Hs Hr]];
+    simpl in Hl; try congruence;
+    simpl; repeat split; congruence.
 Qed.
 
 Lemma EqLimit_move_right : forall n t t',
@@ -128,11 +39,10 @@ Lemma EqLimit_move_right : forall n t t',
   EqLimit (S n) (move_right t) (move_right t').
 Proof.
   introv H.
-  destruct t as [[l s] [u r]].
-  destruct t' as [[l' s'] [u' r']].
-  simpl in H. simpl.
-  destruct H as [El [Es Eur]].
-  repeat split; try assumption; congruence.
+  destruct t as [[l s] r].
+  destruct t' as [[l' s'] r'].
+  destruct H as [Hl [Hs Hr]].
+  simpl. repeat split; congruence.
 Qed.
 
 Local Hint Resolve EqLimit_move_left EqLimit_move_right : core.
@@ -151,7 +61,6 @@ Proof.
   destruct H1 as [H1a [H1b H1c]].
   destruct H2 as [H2a [H2b H2c]].
   repeat split; try congruence.
-  eapply EqTake_trans; eassumption.
 Qed.
 
 Lemma EqLimit_less : forall n k t t',
@@ -159,19 +68,19 @@ Lemma EqLimit_less : forall n k t t',
 Proof.
   intros n k [[l s] r] [[l' s'] r'] H.
   simpl in H. destruct H.
-  eauto.
+  split; eauto.
 Qed.
 
 Local Hint Immediate EqLimit_less : core.
 
 Local Obligation Tactic := program_simplify; intuition.
 
-Program Definition eqb_limit (n : nat) (t t' : ctape)
-    : {EqLimit n (lift_tape t) (lift_tape t')}
-      + {~ EqLimit n (lift_tape t) (lift_tape t')} :=
+Program Definition eqb_limit (n : nat) (t t' : tape)
+    : {EqLimit n t t'} + {~ EqLimit n t t'} :=
   match t, t' with
   | l {{s}} r, l' {{s'}} r' =>
-    eqb_take n l l' && (eqb_sym s s' && Reduce (eqb_side r r'))
+    eqb_side (dfirstn n l) (dfirstn n l') &&
+      (eqb_sym s s' && Reduce (eqb_side r r'))
   end.
 
 (** We define a refinement of the Turing machine step relation,
@@ -215,13 +124,13 @@ Lemma lstep_EqLimit : forall tm k q t1 t2 k' q' t1',
   exists t2', EqLimit k' t1' t2' /\ (k, q;; t2) =[ tm ]=> (k', q';; t2').
 Proof.
   introv Heq Hstep.
-  destruct t1 as [[l1 s1] r1].
-  destruct t2 as [[l2 s2] r2].
+  destruct t1 as [[l s] r].
+  destruct t2 as [[l' s'] r'].
   destruct Heq as [Heq [Es Er]].
-  subst s2 r2. rename s1 into s, r1 into r.
+  subst s' r'.
   inverts Hstep as Htm.
-  - exists (move_left (l2 {{s'}} r)). auto 6.
-  - exists (move_right (l2 {{s'}} r)). auto 6.
+  - exists (move_left (l' {{s'}} r)). auto 6.
+  - exists (move_right (l' {{s'}} r)). auto 6.
 Qed.
 
 Lemma lmultistep_EqLimit : forall tm n k q t1 t2 k' q' t1',
@@ -279,11 +188,11 @@ Proof.
   - auto.
 Qed.
 
-Local Obligation Tactic := program_simplify; autorewrite with core;
+Local Obligation Tactic := program_simplify;
   try (apply lstep_left || apply lstep_right); auto.
 
-Program Definition clstep (tm : TM) (k : nat) (c : Q * ctape)
-    : { '(k', c') | (k, lift c) =[ tm ]=> (k', lift c') } + {True} :=
+Program Definition clstep (tm : TM) (k : nat) (c : Q * tape)
+    : { '(k', c') | (k, c) =[ tm ]=> (k', c') } + {True} :=
   match c with
   | q;; l {{s}} r =>
     match tm (q, s) with
@@ -291,16 +200,16 @@ Program Definition clstep (tm : TM) (k : nat) (c : Q * ctape)
     | Some (s', L, q') =>
       match k with
       | 0 => !!
-      | S k => [|| (k, q';; left (l {{s'}} r)) ||]
+      | S k => [|| (k, q';; move_left (l {{s'}} r)) ||]
       end
-    | Some (s', R, q') => [|| (S k, q';; right (l {{s'}} r)) ||]
+    | Some (s', R, q') => [|| (S k, q';; move_right (l {{s'}} r)) ||]
     end
   end.
 
 Local Obligation Tactic := program_simplify; eauto.
 
-Program Fixpoint clmultistep (tm : TM) (n : nat) (k : nat) (c : Q * ctape)
-    : { '(k', c') | (k, lift c) =[ tm ]=>> n / (k', lift c') } + {True} :=
+Program Fixpoint clmultistep (tm : TM) (n : nat) (k : nat) (c : Q * tape)
+    : { '(k', c') | (k, c) =[ tm ]=>> n / (k', c') } + {True} :=
   match n with
   | 0 => [|| (k, c) ||]
   | S n' =>
@@ -314,7 +223,7 @@ Local Obligation Tactic := program_simplify;
 
 Program Definition verify_tcycler_r (tm : TM) (n0 n1 k : nat)
     : {~ halts tm c0} + {True} :=
-  bind q;; t <- cmultistep tm n0 starting;
+  bind q;; t <- cmultistep tm n0 c0;
   bind (k', q';; t') <- clmultistep tm n1 k (q;; t);
   match n1 with
   | 0 => No
